DP_Proof.thy
@@ -2,11 +2,11 @@ theory DP_Proof
   imports "./DP_CRelVS" "~~/src/HOL/Eisbach/Eisbach_Tools"
 begin           
 
-method dp_match uses induct simp simp\<^sub>T =
-  ( rule dp_consistency.consistentDP_intro,
+method dp_match uses consistency induct simp simp\<^sub>T =
+  ( rule dp_consistency.consistentDP_intro[OF consistency],
     rule induct,
     unfold simp\<^sub>T;
-    rule dp_consistency.crel_vs_checkmem,
+    rule dp_consistency.crel_vs_checkmem[OF consistency],
     unfold simp,
     ((match premises in _[transfer_rule]: _ (multi) \<Rightarrow> transfer_prover)
       | (match conclusion in _ \<Rightarrow> transfer_prover)))
